To simplify the expression \( (P \land \neg Q) \lor (Q \land \neg R) \lor (\neg P \lor R) \), we can follow these steps:

Let's rewrite the expression step-by-step:


   - \( (P \land \neg Q) \) indicates that \( P \) is true and \( Q \) is false.
   - \( (Q \land \neg R) \) indicates that \( Q \) is true and \( R \) is false.
   - \( (\neg P \lor R) \) indicates that either \( P \) is false or \( R \) is true.
### Simplification:

1. **Consider cases**:
   - If \( P \) is true and \( Q \) is false: This satisfies \( (P \land \neg Q) \).
   - If \( Q \) is true and \( R \) is false: This satisfies \( (Q \land \neg R) \).
   - If \( P \) is false, we need \( R \) to be true to satisfy \( (\neg P \lor R) \).

2. **Combine**:
   We can look for overlapping scenarios among these cases. 

However, using a truth table can help visualize this better, leading us to discover potential redundancies. 

### Truth Table:

| P | Q | R | \( P \land \neg Q \) | \( Q \land \neg R \) | \( \neg P \lor R \) | Expression |
|---|---|---|---------------------|---------------------|--------------------|------------|
| T | T | T | F                   | F                   | T                  | T          |
| T | T | F | F                   | T                   | T                  | T          |
| T | F | T | T                   | F                   | T                  | T          |
| T | F | F | T                   | F                   | T                  | T          |
| F | T | T | F                   | F                   | T                  | T          |
| F | T | F | F                   | T                   | T                  | T          |
| F | F | T | F                   | F                   | T                  | T          |
| F | F | F | F                   | F                   | T                  | T          |

### Conclusion:

From the truth table, we see that the entire expression evaluates to true in all scenarios except when \( P \) is true, \( Q \) is true, and \( R \) is false. This means the expression simplifies to:

\[
\neg (P \land Q \land \neg R)
\]

Thus, the simplified version of your original expression is \( \neg (P \land Q \land \neg R) \) or can be expressed in other forms depending on the context needed.