To evaluate the integral \(\iint_R (x - 8y) \, dA\) over the triangular region \(R\) with vertices \((0, 0)\), \((7, 1)\), and \((1, 7)\), using the transformation \(x = 7u + v\) and \(y = u + 7v\), we will follow these steps:

1. **Find the Jacobian of the transformation:**
   We start by calculating the Jacobian determinant \(J\):

   \[
   J = \frac{\partial (x, y)}{\partial (u, v)} = \begin{vmatrix}
   \frac{\partial x}{\partial u} & \frac{\partial x}{\partial v} \\
   \frac{\partial y}{\partial u} & \frac{\partial y}{\partial v}
   \end{vmatrix}
   \]

   First, we compute the partial derivatives:
   \[
   \frac{\partial x}{\partial u} = 7, \quad \frac{\partial x}{\partial v} = 1
   \]
   \[
   \frac{\partial y}{\partial u} = 1, \quad \frac{\partial y}{\partial v} = 7
   \]

   Thus, the Jacobian determinant becomes:
   \[
   J = \begin{vmatrix}
   7 & 1 \\
   1 & 7
   \end{vmatrix} = (7)(7) - (1)(1) = 49 - 1 = 48
   \]

2. **Change of variables in the integral:**
   The integral transforms as follows:
   \[
   \iint*R (x - 8y) \, dA = \iint*{R'} \left((7u + v) - 8(u + 7v)\right) |J| \, du \, dv
   \]
   Simplifying \(x - 8y\):
   \[
   x - 8y = (7u + v) - 8(u + 7v) = 7u + v - 8u - 56v = -u - 55v
   \]

   Therefore, the integral becomes:
   \[
   \iint*{R'} (-u - 55v) (48) \, du \, dv = -48 \iint*{R'} (u + 55v) \, du \, dv
   \]

3. **Find the new region \(R'\):**
   We need to find the vertices of the new triangular region by transforming the original vertices:

   - For \((0, 0)\):
     \[
     u = 0, \, v = 0 \quad \Rightarrow \quad (0, 0)
     \]
   - For \((7, 1)\):
     \[
     7 = 7u + v \quad \text{and} \quad 1 = u + 7v
     \]
     From the first equation, \(v = 7 - 7u\). Substituting into the second:
     \[
     1 = u + 7(7 - 7u) \quad \Rightarrow \quad 1 = u + 49 - 49u \quad \Rightarrow \quad 48u = 48 \quad \Rightarrow \quad u = 1
     \]
     Thus, \(v = 0\). So the vertex \((7, 1)\) maps to \((1, 0)\).

   - For \((1, 7)\):
     \[
     1 = 7u + v \quad \text{and} \quad 7 = u + 7v
     \]
     From the first, \(v = 1 - 7u\). Substituting into the second:
     \[
     7 = u + 7(1 - 7u) \quad \Rightarrow \quad 7 = u + 7 - 49u \quad \Rightarrow \quad 48u = 0 \quad \Rightarrow \quad u = 0
     \]
     Thus, \(v = 1\). So the vertex \((1, 7)\) maps to \((0, 1)\).

   Therefore, the new triangular region \(R'\) has vertices \((0, 0)\), \((1, 0)\), and \((0, 1)\).

4. **Evaluate the transformed integral:**
   The area integral is now:
   \[
   -48 \iint\_{R'} (u + 55v) \, du \, dv
   \]
   The limits for the triangle \(R'\) are \(0 \leq u \leq 1\) and \(0 \leq v \leq 1 - u\):
   \[
   -48 \int_0^1 \int_0^{1-u} (u + 55v) \, dv \, du
   \]

   First, we compute the inner integral:
   \[
   \int_0^{1-u} (u + 55v) \, dv = \left[u v + \frac{55}{2} v^2\right]\_0^{1-u} = u(1-u) + \frac{55}{2}(1-u)^2
   \]
   \[
   = u(1-u) + \frac{55}{2}(1 - 2u + u^2) = u(1-u) + \frac{55}{2} - 55u + \frac{55}{2}u^2
   \]
   \[
   = \left(1 - 55\right) u + \left(1 + \frac{55}{2}\right)u^2 + \frac{55}{2}
   \]

   Next, we integrate with respect to \(u\):
   \[
   -48 \int_0^1 \left(u(1 - 55) + \left(1 + \frac{55}{2}\right)u^2 + \frac{55}{2}\right) \, du
   \]

5. **Calculate the final integral:**
   Now evaluate the integral:
   \[
   -48 \left[ \frac{(1 - 55)}{2}u^2 + \frac{(1 + \frac{55}{2})}{3}u^3 + \frac{55}{2}u \right]\_0^1
   \]

   Plugging in the limits, we will find the value of the entire expression.

To summarize, through the change of variables and careful transformations, we can simplify and evaluate the integral over the new triangular region. The actual evaluation steps may yield a numerical result depending on specific constants.

To evaluate the limits for the integral, we need to explicitly compute the integral:

\[
-48 \int_0^1 \int_0^{1-u} (u + 55v) \, dv \, du.
\]

### Step 1: Evaluate the inner integral

We first compute the inner integral:

\[
\int_0^{1-u} (u + 55v) \, dv.
\]

This can be split into two parts:

\[
\int_0^{1-u} u \, dv + \int_0^{1-u} 55v \, dv.
\]

Calculating each part separately:

1. For the first part:
   \[
   \int_0^{1-u} u \, dv = u \cdot (1-u) = u(1-u).
   \]

2. For the second part:
   \[
   \int_0^{1-u} 55v \, dv = 55 \left[ \frac{v^2}{2} \right]\_0^{1-u} = 55 \cdot \frac{(1-u)^2}{2} = \frac{55}{2}(1-u)^2.
   \]

Combining these results, we have:

\[
\int_0^{1-u} (u + 55v) \, dv = u(1-u) + \frac{55}{2}(1-u)^2.
\]

### Step 2: Evaluate the outer integral

Now we substitute this result into the outer integral:

\[
-48 \int_0^1 \left( u(1-u) + \frac{55}{2}(1-u)^2 \right) \, du.
\]

This separates into two integrals:

\[
-48 \left( \int_0^1 u(1-u) \, du + \frac{55}{2} \int_0^1 (1-u)^2 \, du \right).
\]

#### Evaluating \(\int_0^1 u(1-u) \, du\):

\[
\int_0^1 u(1-u) \, du = \int_0^1 (u - u^2) \, du = \left[ \frac{u^2}{2} - \frac{u^3}{3} \right]\_0^1 = \left( \frac{1}{2} - \frac{1}{3} \right) = \frac{3}{6} - \frac{2}{6} = \frac{1}{6}.
\]

#### Evaluating \(\int_0^1 (1-u)^2 \, du\):

\[
\int_0^1 (1-u)^2 \, du = \int_0^1 (1 - 2u + u^2) \, du = \left[ u - u^2 + \frac{u^3}{3} \right]\_0^1 = \left( 1 - 1 + \frac{1}{3} \right) = \frac{1}{3}.
\]

### Step 3: Combine the results

Now we combine the results of the two integrals:

\[
-48 \left( \frac{1}{6} + \frac{55}{2} \cdot \frac{1}{3} \right) = -48 \left( \frac{1}{6} + \frac{55}{6} \right) = -48 \cdot \frac{56}{6} = -48 \cdot \frac{28}{3} = -16 \cdot 28 = -448.
\]

Thus, the value of the integral is:

\[
\boxed{-448}.
\]

---

---

To evaluate the integral \( \iint_R 2y^2 \, dA \), where \( R \) is the region bounded by the curves \( xy = 4 \), \( xy = 8 \), \( xy^2 = 4 \), and \( xy^2 = 8 \), we can first rewrite the boundaries in terms of \( u \) and \( v \) as given:

- The curves \( xy = 4 \) and \( xy = 8 \) can be expressed as:

  - \( u = 4 \)
  - \( u = 8 \)

- The curves \( xy^2 = 4 \) and \( xy^2 = 8 \) can be expressed as:
  - \( v = 4 \)
  - \( v = 8 \)

### Step 1: Changing Variables

We can set:

- \( u = xy \)
- \( v = xy^2 \)

### Step 2: Find the Jacobian

To change variables, we need the Jacobian \( J \) of the transformation. We compute:

1. From \( u = xy \) and \( v = xy^2 \), we can solve for \( x \) and \( y \):

   - From \( u = xy \), we get \( x = \frac{u}{y} \).
   - Substituting into \( v = xy^2 \), we get \( v = \frac{u}{y} y^2 = uy \) â†’ \( y = \frac{v}{u} \).

2. Substitute \( y \) back into \( x \):
   - \( x = \frac{u}{y} = \frac{u}{\frac{v}{u}} = \frac{u^2}{v} \).

So, we have:
\[
x = \frac{u^2}{v}, \quad y = \frac{v}{u}.
\]

3. Now we compute the Jacobian
\[
\frac{\partial (x,y)}{\partial (u,v)} =
\begin{vmatrix}
\frac{\partial x}{\partial u} & \frac{\partial x}{\partial v} \\
\frac{\partial y}{\partial u} & \frac{\partial y}{\partial v}
\end{vmatrix}
=
\begin{vmatrix}
\frac{2u}{v} & -\frac{u^2}{v^2} \\
-\frac{v}{u^2} & \frac{1}{u}
\end{vmatrix}.
\]

Calculating this determinant:
\[
J = \left(\frac{2u}{v} \cdot \frac{1}{u} \right) - \left(-\frac{u^2}{v^2} \cdot -\frac{v}{u^2}\right) = \frac{2}{v} - \frac{1}{v} = \frac{1}{v}.
\]

### Step 3: Setting up the Integral

Now, the region \( R \) in the \( (u,v) \) plane is bounded by:

- \( 4 \leq u \leq 8 \)
- \( 4 \leq v \leq 8 \)

Thus, the double integral becomes:
\[
\iint_R 2y^2 \, dA = \iint_R 2\left(\frac{v}{u}\right)^2 \left| J \right| \, du \, dv = \iint_R 2\frac{v^2}{u^2} \cdot \frac{1}{v} \, du \, dv = \iint_R \frac{2v}{u^2} \, du \, dv.
\]

### Step 4: Evaluating the Integral

Now we can evaluate:
\[
\int_4^8 \int_4^8 \frac{2v}{u^2} \, du \, dv.
\]

First, evaluate the inner integral with respect to \( u \):
\[
\int_4^8 \frac{2v}{u^2} \, du = 2v \left[-\frac{1}{u}\right]\_4^8 = 2v\left(-\frac{1}{8} + \frac{1}{4}\right) = 2v\left(-\frac{1}{8} + \frac{2}{8}\right) = 2v\left(\frac{1}{8}\right) = \frac{v}{4}.
\]

Now, we integrate with respect to \( v \):
\[
\int_4^8 \frac{v}{4} \, dv = \frac{1}{4} \left[\frac{v^2}{2}\right]\_4^8 = \frac{1}{4} \left(\frac{64}{2} - \frac{16}{2}\right) = \frac{1}{4} \left(32 - 8\right) = \frac{1}{4} \cdot 24 = 6.
\]

### Final Answer

Thus, the value of the integral is:
\[
\boxed{6}.
\]
