To find the equation of the tangent plane to the given parametric surface \( \mathbf{r}(u, v) = u \cos(v) \, \mathbf{i} + u \sin(v) \, \mathbf{j} + v \, \mathbf{k} \) at \( u = 7 \), \( v = \frac{\pi}{3} \), follow these steps:

---

### **Step 1: Compute Partial Derivatives**

The partial derivatives \( \mathbf{r}_u \) and \( \mathbf{r}_v \) give tangent vectors to the surface.

1. **Partial derivative with respect to \( u \):**
   \[
   \mathbf{r}_u = \frac{\partial}{\partial u} \big[ u \cos(v) \, \mathbf{i} + u \sin(v) \, \mathbf{j} + v \, \mathbf{k} \big]
   = \cos(v) \, \mathbf{i} + \sin(v) \, \mathbf{j}
   \]

2. **Partial derivative with respect to \( v \):**
   \[
   \mathbf{r}_v = \frac{\partial}{\partial v} \big[ u \cos(v) \, \mathbf{i} + u \sin(v) \, \mathbf{j} + v \, \mathbf{k} \big]
   = -u \sin(v) \, \mathbf{i} + u \cos(v) \, \mathbf{j} + \mathbf{k}
   \]

---

### **Step 2: Evaluate Partial Derivatives at \( u = 7, v = \frac{\pi}{3} \)**

Substitute \( u = 7 \) and \( v = \frac{\pi}{3} \) into the partial derivatives.

1. **Evaluate \( \mathbf{r}_u \):**
   \[
   \mathbf{r}_u = \cos\left(\frac{\pi}{3}\right) \, \mathbf{i} + \sin\left(\frac{\pi}{3}\right) \, \mathbf{j}
   \]
   Using \( \cos\left(\frac{\pi}{3}\right) = \frac{1}{2} \) and \( \sin\left(\frac{\pi}{3}\right) = \frac{\sqrt{3}}{2} \):
   \[
   \mathbf{r}_u = \frac{1}{2} \, \mathbf{i} + \frac{\sqrt{3}}{2} \, \mathbf{j}
   \]

2. **Evaluate \( \mathbf{r}_v \):**
   \[
   \mathbf{r}_v = -u \sin\left(\frac{\pi}{3}\right) \, \mathbf{i} + u \cos\left(\frac{\pi}{3}\right) \, \mathbf{j} + \mathbf{k}
   \]
   Substituting \( u = 7 \), \( \cos\left(\frac{\pi}{3}\right) = \frac{1}{2} \), and \( \sin\left(\frac{\pi}{3}\right) = \frac{\sqrt{3}}{2} \):
   \[
   \mathbf{r}_v = -7 \cdot \frac{\sqrt{3}}{2} \, \mathbf{i} + 7 \cdot \frac{1}{2} \, \mathbf{j} + \mathbf{k}
   \]
   Simplify:
   \[
   \mathbf{r}_v = -\frac{7\sqrt{3}}{2} \, \mathbf{i} + \frac{7}{2} \, \mathbf{j} + \mathbf{k}
   \]

---

### **Step 3: Compute the Normal Vector**

The normal vector \( \mathbf{N} \) is the cross product of \( \mathbf{r}_u \) and \( \mathbf{r}_v \):
\[
\mathbf{N} = \mathbf{r}_u \times \mathbf{r}_v
\]

1. **Set up the determinant:**
   \[
   \mathbf{N} =
   \begin{vmatrix}
   \mathbf{i} & \mathbf{j} & \mathbf{k} \\
   \frac{1}{2} & \frac{\sqrt{3}}{2} & 0 \\
   -\frac{7\sqrt{3}}{2} & \frac{7}{2} & 1
   \end{vmatrix}
   \]

2. **Expand the determinant:**
   \[
   \mathbf{N} = \mathbf{i} \begin{vmatrix}
   \frac{\sqrt{3}}{2} & 0 \\
   \frac{7}{2} & 1
   \end{vmatrix}
   - \mathbf{j} \begin{vmatrix}
   \frac{1}{2} & 0 \\
   -\frac{7\sqrt{3}}{2} & 1
   \end{vmatrix}
   + \mathbf{k} \begin{vmatrix}
   \frac{1}{2} & \frac{\sqrt{3}}{2} \\
   -\frac{7\sqrt{3}}{2} & \frac{7}{2}
   \end{vmatrix}
   \]

3. **Compute each minor:**
   - For \( \mathbf{i} \):
     \[
     \begin{vmatrix}
     \frac{\sqrt{3}}{2} & 0 \\
     \frac{7}{2} & 1
     \end{vmatrix}
     = \left(\frac{\sqrt{3}}{2} \cdot 1\right) - \left(0 \cdot \frac{7}{2}\right) = \frac{\sqrt{3}}{2}
     \]

   - For \( \mathbf{j} \):
     \[
     \begin{vmatrix}
     \frac{1}{2} & 0 \\
     -\frac{7\sqrt{3}}{2} & 1
     \end{vmatrix}
     = \left(\frac{1}{2} \cdot 1\right) - \left(0 \cdot -\frac{7\sqrt{3}}{2}\right) = \frac{1}{2}
     \]

   - For \( \mathbf{k} \):
     \[
     \begin{vmatrix}
     \frac{1}{2} & \frac{\sqrt{3}}{2} \\
     -\frac{7\sqrt{3}}{2} & \frac{7}{2}
     \end{vmatrix}
     = \left(\frac{1}{2} \cdot \frac{7}{2}\right) - \left(\frac{\sqrt{3}}{2} \cdot -\frac{7\sqrt{3}}{2}\right)
     = \frac{7}{4} + \frac{21}{4} = \frac{28}{4} = 7
     \]

4. **Combine the components:**
   \[
   \mathbf{N} = \frac{\sqrt{3}}{2} \, \mathbf{i} - \frac{1}{2} \, \mathbf{j} + 7 \, \mathbf{k}
   \]

---

### **Step 4: Determine the Point of Tangency**

Substitute \( u = 7 \) and \( v = \frac{\pi}{3} \) into \( \mathbf{r}(u, v) \):
\[
\mathbf{r}(7, \frac{\pi}{3}) = 7 \cos\left(\frac{\pi}{3}\right) \, \mathbf{i} + 7 \sin\left(\frac{\pi}{3}\right) \, \mathbf{j} + \frac{\pi}{3} \, \mathbf{k}
\]
Using \( \cos\left(\frac{\pi}{3}\right) = \frac{1}{2} \) and \( \sin\left(\frac{\pi}{3}\right) = \frac{\sqrt{3}}{2} \):
\[
\mathbf{r}(7, \frac{\pi}{3}) = \frac{7}{2} \, \mathbf{i} + \frac{7\sqrt{3}}{2} \, \mathbf{j} + \frac{\pi}{3} \, \mathbf{k}
\]
Thus, \( \mathbf{P}_0 = \left( \frac{7}{2}, \frac{7\sqrt{3}}{2}, \frac{\pi}{3} \right) \).

---

### **Step 5: Write the Tangent Plane Equation**

Using the point-normal form of a plane:
\[
\mathbf{N} \cdot (\mathbf{X} - \mathbf{P}_0) = 0
\]
Let \( \mathbf{X} = \langle x, y, z \rangle \) and \( \mathbf{P}_0 = \left( \frac{7}{2}, \frac{7\sqrt{3}}{2}, \frac{\pi}{3} \right) \). Expand:
\[
\frac{\sqrt{3}}{2}(x - \frac{7}{2}) - \frac{1}{2}(y - \

frac{7\sqrt{3}}{2}) + 7(z - \frac{\pi}{3}) = 0
\]

Simplify:
\[
\frac{\sqrt{3}}{2}x - \frac{7\sqrt{3}}{4} - \frac{1}{2}y + \frac{7\sqrt{3}}{4} + 7z - \frac{7\pi}{3} = 0
\]

Combine terms:
\[
\frac{\sqrt{3}}{2}x - \frac{1}{2}y + 7z - \frac{7\pi}{3} = 0
\]

---

### **Final Answer:**
\[
\frac{\sqrt{3}}{2}x - \frac{1}{2}y + 7z = \frac{7\pi}{3}
\]